Prove upto context and compatibility

src/lang/Configuration.v
@@ -14,36 +14,37 @@ Set Implicit Arguments.
 
 
 Module Configuration.
-  Definition syntax := IdentMap.t State.syntax.
+  Definition syntax := IdentMap.t {lang:Language.t & lang.(Language.syntax)}.
 
   Structure t := mk {
-    threads: IdentMap.t Thread.t;
+    threads: IdentMap.t {lang:Language.t & Thread.t lang};
     memory: Memory.t;
   }.
 
   Definition init (s:syntax): t :=
-    mk (IdentMap.map Thread.init s) Memory.init.
+    mk (IdentMap.map (fun s => existT _ _ (Thread.init _ s.(projT2))) s)
+       Memory.init.
 
   Definition is_terminal (conf:t): Prop :=
-    forall tid th (FIND: IdentMap.find tid conf.(threads) = Some th),
-      Thread.is_terminal th.
+    forall tid lang st (FIND: IdentMap.find tid conf.(threads) = Some (existT _ lang st)),
+      Thread.is_terminal st.
 
   Inductive step (e:option Event.t) (c1:t): forall (c2:t), Prop :=
   | step_intro
-      tid th1 th2 memory2 th3 memory3
-      (TID: IdentMap.find tid c1.(threads) = Some th1)
-      (STEPS: rtc Thread.internal_step (th1, c1.(memory)) (th2, memory2))
+      tid lang th1 th2 memory2 th3 memory3
+      (TID: IdentMap.find tid c1.(threads) = Some (existT _ lang th1))
+      (STEPS: rtc (@Thread.internal_step lang) (th1, c1.(memory)) (th2, memory2))
       (STEP: Thread.step e th2 memory2 th3 memory3)
       (CONSISTENT: Thread.consistent th3 memory3):
-      step e c1 (mk (IdentMap.add tid th3 c1.(threads)) memory3)
+      step e c1 (mk (IdentMap.add tid (existT _ _ th3) c1.(threads)) memory3)
   .
 
   Definition consistent (conf:t): Prop :=
-    forall tid th1 mem1
-      (FIND: IdentMap.find tid conf.(threads) = Some th1)
+    forall tid lang th1 mem1
+      (FIND: IdentMap.find tid conf.(threads) = Some (existT _ lang th1))
       (LOCAL: Memory.le th1.(Thread.local) mem1)
       (FUTURE: Memory.future conf.(memory) mem1),
     exists th2 mem2,
-      <<STEPS: rtc Thread.internal_step (th1, mem1) (th2, mem2)>> /\
+      <<STEPS: rtc (@Thread.internal_step lang) (th1, mem1) (th2, mem2)>> /\
       <<DECLARE: th2.(Thread.local) = Memory.init>>.
 End Configuration.
