src/lang/Language.v
@@ -1,5 +1,6 @@
 Require Import sflib.
 
+Require Import Axioms.
 Require Import Basic.
 Require Import Event.
 Require Import Time.
@@ -16,27 +17,3 @@ Module Language.
     step: forall (s1:state) (e:option ThreadEvent.t) (s2:state), Prop;
   }.
 End Language.
-
-Module State.
-  Structure syntax := mk_syntax {
-    syntax_lang: Language.t;
-    syntax_syntax: syntax_lang.(Language.syntax);
-  }.
-
-  Structure t := mk {
-    lang: Language.t;
-    state: lang.(Language.state)
-  }.
-
-  Definition init (s:syntax): t :=
-    mk s.(syntax_lang) (s.(syntax_lang).(Language.init) s.(syntax_syntax)).
-
-  Definition is_terminal (th:t): Prop :=
-    th.(lang).(Language.is_terminal) th.(state).
-
-  Inductive step: forall (t1:t) (e:option ThreadEvent.t) (t2:t), Prop :=
-  | step_intro
-      lang s1 e s2
-      (STEP: lang.(Language.step) s1 e s2):
-      step (mk lang s1) e (mk lang s2).
-End State.
