src/lang/Thread.v
@@ -76,135 +76,147 @@ Module Commit.
 End Commit.
 
 Module Thread.
-  Structure t := mk {
-    state: State.t;
-    commit: Commit.t;
-    local: Memory.t;
-  }.
+  Section Thread.
+    Variable (lang:Language.t).
 
-  Definition init (s:State.syntax) := mk (State.init s) Commit.init Memory.init.
+    Definition syntax := lang.(Language.syntax).
 
-  Inductive is_terminal (th:t): Prop :=
-  | is_terminal_intro
-      (STATE: State.is_terminal th.(state))
-      (LOCAL: th.(local) = Memory.init)
-  .
+    Structure t := mk {
+      state: lang.(Language.state);
+      commit: Commit.t;
+      local: Memory.t;
+    }.
 
-  Inductive memory_step (th1:t) (mem1:Memory.t): forall (th2:t), Prop :=
-  | step_read
-      loc val ts released ord st2 commit2
-      (STATE: State.step th1.(state) (Some (ThreadEvent.mem (MemEvent.read loc val ord))) st2)
-      (READ: Commit.read th1.(commit) loc ts released ord commit2)
-      (MESSAGE: Memory.get loc ts mem1 = Some (Message.mk val released))
-      (LOCAL: Memory.get loc ts th1.(local) = None):
-      memory_step th1 mem1
-                  (mk st2 commit2 th1.(local))
-  | step_write
-      loc val ts released ord st2 commit2
-      (STATE: State.step th1.(state) (Some (ThreadEvent.mem (MemEvent.write loc val ord))) st2)
-      (WRITE: Commit.write th1.(commit) loc ts released ord commit2)
-      (MESSAGE: Memory.get loc ts th1.(local) = Some (Message.mk val released)):
-      memory_step th1 mem1
-                  (mk st2 commit2 (Memory.remove loc ts th1.(local)))
-  | step_update
-      loc valr tsr releasedr valw tsw releasedw ord st3 commit2 commit3
-      (STATE: State.step th1.(state) (Some (ThreadEvent.mem (MemEvent.update loc valr valw ord))) st3)
-      (READ: Commit.read th1.(commit) loc tsr releasedr ord commit2)
-      (WRITE: Commit.write commit2 loc tsw releasedw ord commit3)
-      (RELEASE: Snapshot.le releasedr releasedw)
-      (MESSAGE1: Memory.get loc tsr mem1 = Some (Message.mk valr releasedr))
-      (MESSAGE2: Memory.get loc tsw th1.(local) = Some (Message.mk valw releasedw)):
-      memory_step th1 mem1
-                  (mk st3 commit3 (Memory.remove loc tsw th1.(local)))
-  | step_fence
-      ord st2 commit2
-      (STATE: State.step th1.(state) (Some (ThreadEvent.mem (MemEvent.fence ord))) st2)
-      (FENCE: Commit.fence th1.(commit) ord commit2):
-      memory_step th1 mem1
-                  (mk st2 commit2 th1.(local))
-  | step_None
-      commit2
-      (COMMIT: Commit.le th1.(commit) commit2):
-      memory_step th1 mem1
-                  (mk th1.(state) commit2 th1.(local))
-  .
+    Definition init (s:syntax) :=
+      mk (lang.(Language.init) s)
+         Commit.init
+         Memory.init.
 
-  Inductive declare_step (th1:t) (mem1:Memory.t) (th2:t) (mem2:Memory.t): Prop :=
-  | declare_step_intro
-      loc from to msg
-      (STATE: th1.(state) = th2.(state))
-      (COMMIT: Commit.le th1.(commit) th2.(commit))
-      (LOCAL: Memory.declare loc from to msg th1.(local) th2.(local))
-      (MEMORY: Memory.declare loc from to msg mem1 mem2)
-  .
+    Inductive is_terminal (th:t): Prop :=
+    | is_terminal_intro
+        (STATE: lang.(Language.is_terminal) th.(state))
+        (LOCAL: th.(local) = Memory.init)
+    .
 
-  Inductive step: forall (e:option Event.t) (th1:t) (mem1:Memory.t) (th2:t) (mem2:Memory.t), Prop :=
-  | step_memory
-      th1 th2 mem
-      (STEP: memory_step th1 mem th2):
-      step None th1 mem th2 mem
-  | step_declare
-      th1 mem1 th2 mem2
-      (STEP: declare_step th1 mem1 th2 mem2):
-      step None th1 mem1 th2 mem2
-  | step_external
-      st1 st2 commit1 commit2 mem e
-      (STATE: State.step st1 (Some (ThreadEvent.syscall e)) st2)
-      (COMMIT: Commit.le commit1 commit2):
-      step (Some e)
-           (mk st1 commit1 Memory.init) mem
-           (mk st2 commit2 Memory.init) mem
-  .
+    Inductive memory_step (th1:t) (mem1:Memory.t): forall (th2:t), Prop :=
+    | step_read
+        loc val ts released ord st2 commit2
+        (STATE: lang.(Language.step) th1.(state) (Some (ThreadEvent.mem (MemEvent.read loc val ord))) st2)
+        (READ: Commit.read th1.(commit) loc ts released ord commit2)
+        (MESSAGE: Memory.get loc ts mem1 = Some (Message.mk val released))
+        (LOCAL: Memory.get loc ts th1.(local) = None):
+        memory_step th1 mem1
+                    (mk st2 commit2 th1.(local))
+    | step_write
+        loc val ts released ord st2 commit2
+        (STATE: lang.(Language.step) th1.(state) (Some (ThreadEvent.mem (MemEvent.write loc val ord))) st2)
+        (WRITE: Commit.write th1.(commit) loc ts released ord commit2)
+        (MESSAGE: Memory.get loc ts th1.(local) = Some (Message.mk val released)):
+        memory_step th1 mem1
+                    (mk st2 commit2 (Memory.remove loc ts th1.(local)))
+    | step_update
+        loc valr tsr releasedr valw tsw releasedw ord st3 commit2 commit3
+        (STATE: lang.(Language.step) th1.(state) (Some (ThreadEvent.mem (MemEvent.update loc valr valw ord))) st3)
+        (READ: Commit.read th1.(commit) loc tsr releasedr ord commit2)
+        (WRITE: Commit.write commit2 loc tsw releasedw ord commit3)
+        (RELEASE: Snapshot.le releasedr releasedw)
+        (MESSAGE1: Memory.get loc tsr mem1 = Some (Message.mk valr releasedr))
+        (MESSAGE2: Memory.get loc tsw th1.(local) = Some (Message.mk valw releasedw)):
+        memory_step th1 mem1
+                    (mk st3 commit3 (Memory.remove loc tsw th1.(local)))
+    | step_fence
+        ord st2 commit2
+        (STATE: lang.(Language.step) th1.(state) (Some (ThreadEvent.mem (MemEvent.fence ord))) st2)
+        (FENCE: Commit.fence th1.(commit) ord commit2):
+        memory_step th1 mem1
+                    (mk st2 commit2 th1.(local))
+    | step_None
+        st2 commit2
+        (STATE: lang.(Language.step) th1.(state) None st2)
+        (COMMIT: Commit.le th1.(commit) commit2):
+        memory_step th1 mem1
+                    (mk st2 commit2 th1.(local))
+    .
 
-  Inductive internal_step (c1 c2:t * Memory.t): Prop :=
-  | internal_step_intro
-      (STEP: step None c1.(fst) c1.(snd) c2.(fst) c2.(snd))
-  .
+    Inductive declare_step (th1:t) (mem1:Memory.t): forall (th2:t) (mem2:Memory.t), Prop :=
+    | declare_step_intro
+        loc from to msg st2 commit2 local2 mem2
+        (STATE: th1.(state) = st2)
+        (COMMIT: Commit.le th1.(commit) commit2)
+        (LOCAL: Memory.declare loc from to msg th1.(local) local2)
+        (MEMORY: Memory.declare loc from to msg mem1 mem2):
+        declare_step th1 mem1
+                     (mk st2 commit2 local2) mem2
+    .
 
-  Definition consistent (th1:t) (mem:Memory.t): Prop :=
-    forall mem1
-      (LOCAL: Memory.le th1.(Thread.local) mem1)
-      (FUTURE: Memory.future mem mem1),
-    exists th2 mem2,
-      <<STEPS: rtc internal_step (th1, mem1) (th2, mem2)>> /\
-      <<DECLARE: th2.(Thread.local) = Memory.init>>.
+    Inductive step: forall (e:option Event.t) (th1:t) (mem1:Memory.t) (th2:t) (mem2:Memory.t), Prop :=
+    | step_memory
+        th1 th2 mem
+        (STEP: memory_step th1 mem th2):
+        step None th1 mem th2 mem
+    | step_declare
+        th1 mem1 th2 mem2
+        (STEP: declare_step th1 mem1 th2 mem2):
+        step None th1 mem1 th2 mem2
+    | step_external
+        st1 st2 commit1 commit2 mem e
+        (STATE: lang.(Language.step) st1 (Some (ThreadEvent.syscall e)) st2)
+        (COMMIT: Commit.le commit1 commit2):
+        step (Some e)
+             (mk st1 commit1 Memory.init) mem
+             (mk st2 commit2 Memory.init) mem
+    .
 
-  Lemma disjoint_memory_step
-        th1 mem1 th2 mem_o
-        (STEP: memory_step th1 mem1 th2)
-        (DISJOINT: Memory.disjoint mem_o th1.(local))
-        (LE: Memory.le mem_o mem1):
-    Memory.disjoint mem_o th2.(local).
-  Proof.
-    inv STEP; simpl in *; auto.
-    - admit.
-    - admit.
-  Admitted.
+    Inductive internal_step (c1 c2:t * Memory.t): Prop :=
+    | internal_step_intro
+        (STEP: step None c1.(fst) c1.(snd) c2.(fst) c2.(snd))
+    .
 
-  Lemma disjoint_declare_step
-        th1 mem1 th2 mem2 mem_o
-        (STEP: declare_step th1 mem1 th2 mem2)
-        (DISJOINT: Memory.disjoint mem_o th1.(local))
-        (LE: Memory.le mem_o mem1):
-    <<DISJOINT: Memory.disjoint mem_o th2.(local)>> /\
-    <<LE: Memory.le mem_o mem2>>.
-  Proof.
-    inv STEP.
-    admit.
-  Admitted.
+    Definition consistent (th1:t) (mem:Memory.t): Prop :=
+      forall mem1
+        (LOCAL: Memory.le th1.(local) mem1)
+        (FUTURE: Memory.future mem mem1),
+      exists th2 mem2,
+        <<STEPS: rtc internal_step (th1, mem1) (th2, mem2)>> /\
+        <<DECLARE: th2.(local) = Memory.init>>.
 
-  Lemma disjoint_step
-        th1 mem1 th2 mem2 e mem_o
-        (STEP: step e th1 mem1 th2 mem2)
-        (DISJOINT: Memory.disjoint mem_o th1.(local))
-        (LE: Memory.le mem_o mem1):
-    <<DISJOINT: Memory.disjoint mem_o th2.(local)>> /\
-    <<LE: Memory.le mem_o mem2>>.
-  Proof.
-    inv STEP.
-    - splits; auto.
-      eapply disjoint_memory_step; eauto.
-    - eapply disjoint_declare_step; eauto.
-    - simpl in *. splits; auto.
-  Qed.
+    Lemma disjoint_memory_step
+          th1 mem1 th2 mem_o
+          (STEP: memory_step th1 mem1 th2)
+          (DISJOINT: Memory.disjoint mem_o th1.(local))
+          (LE: Memory.le mem_o mem1):
+      Memory.disjoint mem_o th2.(local).
+    Proof.
+      inv STEP; simpl in *; auto.
+      - admit.
+      - admit.
+    Admitted.
+
+    Lemma disjoint_declare_step
+          th1 mem1 th2 mem2 mem_o
+          (STEP: declare_step th1 mem1 th2 mem2)
+          (DISJOINT: Memory.disjoint mem_o th1.(local))
+          (LE: Memory.le mem_o mem1):
+      <<DISJOINT: Memory.disjoint mem_o th2.(local)>> /\
+                  <<LE: Memory.le mem_o mem2>>.
+    Proof.
+      inv STEP.
+      admit.
+    Admitted.
+
+    Lemma disjoint_step
+          th1 mem1 th2 mem2 e mem_o
+          (STEP: step e th1 mem1 th2 mem2)
+          (DISJOINT: Memory.disjoint mem_o th1.(local))
+          (LE: Memory.le mem_o mem1):
+      <<DISJOINT: Memory.disjoint mem_o th2.(local)>> /\
+                  <<LE: Memory.le mem_o mem2>>.
+    Proof.
+      inv STEP.
+      - splits; auto.
+        eapply disjoint_memory_step; eauto.
+      - eapply disjoint_declare_step; eauto.
+      - simpl in *. splits; auto.
+    Qed.
+  End Thread.
 End Thread.
