src/opt/Compatibility.v
@@ -1,0 +1,466 @@
+Require Import Basics.
+Require Import Bool.
+Require Import List.
+
+Require Import sflib.
+Require Import paco.
+Require Import respectful5.
+
+Require Import Axioms.
+Require Import Basic.
+Require Import Event.
+Require Import Language.
+Require Import Memory.
+Require Import Thread.
+Require Import Configuration.
+Require Import Simulation.
+
+Require Import Syntax.
+Require Import Semantics.
+
+Set Implicit Arguments.
+
+Definition SIM_REGS := forall (rs_src rs_tgt:RegFile.t), Prop.
+
+Inductive sim_terminal
+          (sim_regs:SIM_REGS)
+          (th_src th_tgt:Thread.t lang): Prop :=
+| sim_terminal_intro
+    (REGS: sim_regs th_src.(Thread.state).(State.regs) th_tgt.(Thread.state).(State.regs))
+    (COMMIT: th_src.(Thread.commit) = th_tgt.(Thread.commit))
+.
+
+Definition sim_expr
+           (sim_regs:SIM_REGS)
+           e_src e_tgt :=
+  forall rs_src rs_tgt (RS: sim_regs rs_src rs_tgt),
+    RegFile.eval_expr rs_src e_src = RegFile.eval_expr rs_tgt e_tgt.
+
+Definition _sim_stmts
+           (sim_thread:SIM_THREAD lang)
+           (sim_regs0:SIM_REGS)
+           (stmts_src stmts_tgt:list Stmt.t)
+           (sim_regs1:SIM_REGS): Prop :=
+  forall rs_src rs_tgt commit local mem_k_src mem_k_tgt
+    (RS: sim_regs0 rs_src rs_tgt),
+    sim_thread
+      (sim_terminal sim_regs1)
+      (Thread.mk lang (State.mk rs_src stmts_src) commit local) mem_k_src
+      (Thread.mk lang (State.mk rs_tgt stmts_tgt) commit local) mem_k_tgt.
+
+Lemma _sim_stmts_mon
+      s1 s2 (S: s1 <5= s2):
+  _sim_stmts s1 <4= _sim_stmts s2.
+Proof.
+  ii. apply S. apply PR. auto.
+Qed.
+
+Lemma step_seq
+      stmts rs1 stmts1 rs2 stmts2 e
+      (STEP: State.step (State.mk rs1 stmts1) e
+                        (State.mk rs2 stmts2)):
+  State.step (State.mk rs1 (stmts1 ++ stmts)) e
+             (State.mk rs2 (stmts2 ++ stmts)).
+Proof.
+  inv STEP.
+  - econs 1. auto.
+  - simpl. rewrite <- app_assoc. econs 2.
+  - simpl. rewrite <- app_assoc. econs 3.
+Qed.
+
+Lemma step_deseq
+      stmts rs1 stmt1 stmts1 rs2 stmts2 e
+      (STEP: State.step (State.mk rs1 (stmt1 :: stmts1 ++ stmts)) e
+                        (State.mk rs2 stmts2)):
+  exists stmts2',
+    stmts2 = stmts2' ++ stmts /\
+    State.step (State.mk rs1 (stmt1 :: stmts1)) e
+               (State.mk rs2 stmts2').
+Proof.
+  inv STEP.
+  - eexists. splits; eauto. econs 1. auto.
+  - eexists. rewrite app_assoc. splits; eauto. econs 2.
+  - eexists. rewrite app_comm_cons, app_assoc. splits; eauto. econs 3.
+Qed.
+
+Lemma thread_step_seq
+      stmts e
+      rs1 stmts1 commit1 local1 mem1
+      rs2 stmts2 commit2 local2 mem2
+      (STEP: Thread.step e
+               (Thread.mk lang (State.mk rs1 stmts1) commit1 local1) mem1
+               (Thread.mk lang (State.mk rs2 stmts2) commit2 local2) mem2):
+  Thread.step e
+    (Thread.mk lang (State.mk rs1 (stmts1 ++ stmts)) commit1 local1) mem1
+    (Thread.mk lang (State.mk rs2 (stmts2 ++ stmts)) commit2 local2) mem2.
+Proof.
+  inv STEP.
+  - econs 1. inv STEP0; simpl in *.
+    + econs 1; simpl; eauto. apply step_seq. auto.
+    + econs 2; simpl; eauto. apply step_seq. auto.
+    + econs 3; simpl; eauto. apply step_seq. auto.
+    + econs 4; simpl; eauto. apply step_seq. auto.
+    + econs 5; simpl; eauto. apply step_seq. auto.
+  - econs 2. inv STEP0. inv STATE. simpl in *.
+    econs; eauto.
+  - econs 3; eauto. inv STATE. econs; eauto.
+Qed.
+
+Lemma internal_step_seq
+      stmts
+      rs1 stmts1 commit1 local1 mem1
+      rs2 stmts2 commit2 local2 mem2
+      (STEP: Thread.internal_step
+               (Thread.mk lang (State.mk rs1 stmts1) commit1 local1, mem1)
+               (Thread.mk lang (State.mk rs2 stmts2) commit2 local2, mem2)):
+  Thread.internal_step
+    (Thread.mk lang (State.mk rs1 (stmts1 ++ stmts)) commit1 local1, mem1)
+    (Thread.mk lang (State.mk rs2 (stmts2 ++ stmts)) commit2 local2, mem2).
+Proof.
+  econs. simpl in *.
+  eapply thread_step_seq; eauto.
+  inv STEP; eauto.
+Qed.
+
+Lemma thread_step_deseq
+      stmts e
+      rs1 stmt1 stmts1 commit1 local1 mem1
+      rs2 stmts2 commit2 local2 mem2
+      (STEP: Thread.step e
+                         (Thread.mk lang (State.mk rs1 (stmt1 :: stmts1 ++ stmts)) commit1 local1) mem1
+                         (Thread.mk lang (State.mk rs2 stmts2) commit2 local2) mem2):
+  exists stmts2',
+    stmts2 = stmts2' ++ stmts /\
+  Thread.step e
+              (Thread.mk lang (State.mk rs1 (stmt1 :: stmts1)) commit1 local1) mem1
+              (Thread.mk lang (State.mk rs2 stmts2') commit2 local2) mem2.
+Proof.
+  inv STEP.
+  - inv STEP0; simpl in *.
+    + apply step_deseq in STATE. des. subst.
+      eexists. splits; eauto.
+      econs 1. econs 1; simpl; eauto.
+    + apply step_deseq in STATE. des. subst.
+      eexists. splits; eauto.
+      econs 1. econs 2; simpl; eauto.
+    + apply step_deseq in STATE. des. subst.
+      eexists. splits; eauto.
+      econs 1. econs 3; simpl; eauto.
+    + apply step_deseq in STATE. des. subst.
+      eexists. splits; eauto.
+      econs 1. econs 4; simpl; eauto.
+    + apply step_deseq in STATE. des. subst.
+      eexists. splits; eauto.
+      econs 1. econs 5; simpl; eauto.
+  - inv STEP0; simpl in *.
+    inv STATE.
+    rewrite app_comm_cons.
+    eexists. splits; eauto.
+    econs 2. econs; eauto.
+  - inv STATE.
+    eexists. splits; eauto.
+    econs 3; eauto. econs; eauto.
+Qed.
+
+Lemma rtc_sim
+      A B
+      (sim:A -> B -> Prop)
+      (rA:A -> A -> Prop)
+      (rB:B -> B -> Prop)
+      (SIM:
+         forall a1 a2 b1 (RA: rA a1 a2) (SIM1: sim a1 b1),
+         exists b2, rB b1 b2 /\ sim a2 b2)
+      a1 a2 b1
+      (RA: rtc rA a1 a2) (SIM1: sim a1 b1):
+  exists b2, rtc rB b1 b2 /\ sim a2 b2.
+Proof.
+  revert b1 SIM1. induction RA; i.
+  - eexists. splits; eauto.
+  - exploit SIM; eauto. i. des.
+    exploit IHRA; eauto. i. des.
+    eexists. splits; [|eauto].
+    econs; eauto.
+Qed.
+
+Inductive sim_seq (s:list Stmt.t): forall (lhs rhs:Thread.t lang * Memory.t), Prop :=
+| sim_seq_intro
+    rs stmts commit local mem:
+    sim_seq s
+            (Thread.mk lang (State.mk rs stmts) commit local, mem)
+            (Thread.mk lang (State.mk rs (stmts ++ s)) commit local, mem)
+.
+
+Lemma rtc_internal_step_seq
+      stmts
+      rs1 stmts1 commit1 local1 mem1
+      rs2 stmts2 commit2 local2 mem2
+      (STEP: rtc (@Thread.internal_step lang)
+               (Thread.mk lang (State.mk rs1 stmts1) commit1 local1, mem1)
+               (Thread.mk lang (State.mk rs2 stmts2) commit2 local2, mem2)):
+  rtc (@Thread.internal_step lang)
+    (Thread.mk lang (State.mk rs1 (stmts1 ++ stmts)) commit1 local1, mem1)
+    (Thread.mk lang (State.mk rs2 (stmts2 ++ stmts)) commit2 local2, mem2).
+Proof.
+  exploit (rtc_sim (sim_seq stmts)); eauto.
+  - i. inv SIM1. inv RA. simpl in *.
+    destruct a2. destruct t. destruct state. simpl in *.
+    exploit internal_step_seq; eauto. i.
+    eexists. splits; eauto. econs; eauto.
+  - econs; eauto.
+  - i. des. inv x1. auto.
+Unshelve.
+  { econs; auto. }
+Qed.
+
+Inductive ctx (sim_thread:SIM_THREAD lang): SIM_THREAD lang :=
+| ctx_incl
+    sim_terminal
+    th1 mem_k_src th2 mem_k_tgt
+    (SIM: sim_thread sim_terminal th1 mem_k_src th2 mem_k_tgt):
+    ctx sim_thread sim_terminal th1 mem_k_src th2 mem_k_tgt
+| ctx_nil
+    (sim_regs:SIM_REGS)
+    rs_src mem_k_src
+    rs_tgt mem_k_tgt
+    commit local
+    (RS: sim_regs rs_src rs_tgt):
+    ctx sim_thread
+        (sim_terminal sim_regs)
+        (Thread.mk lang (State.mk rs_src nil) commit local) mem_k_src
+        (Thread.mk lang (State.mk rs_tgt nil) commit local) mem_k_tgt
+| ctx_instr
+    (sim_regs:SIM_REGS)
+    instr
+    (REGS: forall reg (REG: RegSet.mem reg (Instr.regs_of instr))
+             rs_src rs_tgt (RS: sim_regs rs_src rs_tgt),
+        rs_src reg = rs_tgt reg)
+    rs_src mem_k_src
+    rs_tgt mem_k_tgt
+    commit local
+    (RS: sim_regs rs_src rs_tgt):
+    ctx sim_thread
+        (sim_terminal sim_regs)
+        (Thread.mk lang (State.mk rs_src [Stmt.instr instr]) commit local) mem_k_src
+        (Thread.mk lang (State.mk rs_tgt [Stmt.instr instr]) commit local) mem_k_tgt
+| ctx_seq
+    sim_regs1 sim_regs2
+    stmts1_src stmts2_src rs_src commit_src local_src mem_k_src
+    stmts1_tgt stmts2_tgt rs_tgt commit_tgt local_tgt mem_k_tgt
+    (SIM1: sim_thread (sim_terminal sim_regs1)
+                      (Thread.mk lang (State.mk rs_src stmts1_src) commit_src local_src) mem_k_src
+                      (Thread.mk lang (State.mk rs_tgt stmts1_tgt) commit_tgt local_tgt) mem_k_tgt)
+    (SIM2: _sim_stmts sim_thread sim_regs1 stmts2_src stmts2_tgt sim_regs2):
+    ctx sim_thread
+        (sim_terminal sim_regs2)
+        (Thread.mk lang (State.mk rs_src (stmts1_src ++ stmts2_src)) commit_src local_src) mem_k_src
+        (Thread.mk lang (State.mk rs_tgt (stmts1_tgt ++ stmts2_tgt)) commit_tgt local_tgt) mem_k_tgt
+| ctx_ite
+    sim_regs0 sim_regs1
+    cond_src stmts1_src stmts2_src rs_src mem_k_src
+    cond_tgt stmts1_tgt stmts2_tgt rs_tgt mem_k_tgt
+    commit local
+    (COND: sim_expr sim_regs0 cond_src cond_tgt)
+    (RS: sim_regs0 rs_src rs_tgt)
+    (SIM1: _sim_stmts sim_thread sim_regs0 stmts1_src stmts1_tgt sim_regs1)
+    (SIM2: _sim_stmts sim_thread sim_regs0 stmts2_src stmts2_tgt sim_regs1):
+    ctx sim_thread
+        (sim_terminal sim_regs1)
+        (Thread.mk lang (State.mk rs_src [Stmt.ite cond_src stmts1_src stmts2_src]) commit local) mem_k_src
+        (Thread.mk lang (State.mk rs_tgt [Stmt.ite cond_tgt stmts1_tgt stmts2_tgt]) commit local) mem_k_tgt
+| ctx_dowhile
+    sim_regs
+    cond_src stmts_src rs_src mem_k_src
+    cond_tgt stmts_tgt rs_tgt mem_k_tgt
+    commit local
+    (COND: sim_expr sim_regs cond_src cond_tgt)
+    (RS: sim_regs rs_src rs_tgt)
+    (SIM: _sim_stmts sim_thread sim_regs stmts_src stmts_tgt sim_regs):
+    ctx sim_thread
+        (sim_terminal sim_regs)
+        (Thread.mk lang (State.mk rs_src [Stmt.dowhile stmts_src cond_src]) commit local) mem_k_src
+        (Thread.mk lang (State.mk rs_tgt [Stmt.dowhile stmts_tgt cond_tgt]) commit local) mem_k_tgt
+.
+Hint Constructors ctx.
+
+Lemma ctx_mon: monotone5 ctx.
+Proof.
+  ii. inv IN.
+  - econs 1. auto.
+  - econs 2. auto.
+  - econs 3; eauto; eapply _sim_stmts_mon; eauto.
+  - econs 4; eauto; eapply _sim_stmts_mon; eauto.
+  - econs 5; eauto; eapply _sim_stmts_mon; eauto.
+  - econs 6; eauto; eapply _sim_stmts_mon; eauto.
+Qed.
+Hint Resolve ctx_mon.
+
+Lemma ctx_weak_respectful: weak_respectful5 (@_sim_thread lang) ctx.
+Proof.
+  econs; auto. i. destruct PR.
+  - (* incl *)
+    eapply _sim_thread_mon; eauto.
+    apply rclo5_incl.
+  - (* nil *)
+    ii. splits.
+    { i. inv TERMINAL_TGT. simpl in *.
+      eexists _, _. splits; eauto; econs; simpl; auto.
+    }
+    { i. simpl in *. subst.
+      eexists _, _. splits; eauto; econs; simpl; auto.
+    }
+    i. inv STEP_TGT; simpl in *.
+    + inv STEP; inv STATE.
+    + admit. (* declare *)
+    + inv STATE.
+  - (* instr *)
+    ii. splits.
+    { i. inv TERMINAL_TGT. }
+    { i. simpl in *. subst. eexists _, _. splits; eauto. }
+    i. inv STEP_TGT; simpl in *.
+    + inv STEP; simpl in *; inv STATE.
+      * admit. (* load *)
+      * admit. (* store *)
+      * admit. (* update *)
+      * admit. (* fence *)
+      * admit. (* None *)
+    + admit. (* declare *)
+    + admit. (* syscall *)
+  - (* seq *)
+    ii. simpl in *.
+    exploit GF; eauto. simpl. i. des.
+    splits.
+    { i. inv TERMINAL_TGT. destruct stmts1_tgt, stmts2_tgt; inv H0.
+      exploit TERMINAL; try by econs. i. des.
+      destruct th2_src, state. inv TERMINAL_SRC. simpl in *. subst.
+      inv SIM. simpl in *. subst.
+      exploit SIM2; eauto. intro TH2.
+      exploit GF; eauto.
+      { admit. (* memory le *) }
+      { admit. (* memory future *)  }
+      i. des.
+      exploit TERMINAL0; try by econs. i. des.
+      destruct th2_src, state. inv TERMINAL_SRC. simpl in *. subst.
+      eexists _, _. splits; [|eauto| | |eauto].
+      + eapply rtc_trans; [|eauto].
+        eapply rtc_internal_step_seq in STEPS. apply STEPS.
+      + econs.
+      + econs.
+    }
+    { i. subst. exploit DECLARE; eauto. i. des.
+      destruct th2_src, state. simpl in *. subst.
+      eexists _, _. splits; [|eauto|eauto].
+      + eapply rtc_internal_step_seq. apply STEPS.
+      + eauto.
+    }
+    destruct stmts1_tgt.
+    + i. exploit TERMINAL; try by econs. i. des.
+      destruct th2_src, state. inv TERMINAL_SRC. simpl in *. subst.
+      inv SIM. simpl in *. subst.
+      exploit SIM2; eauto. intro TH2.
+      exploit GF; eauto.
+      { admit. (* memory le *) }
+      { admit. (* memory future *)  }
+      i. des.
+      exploit STEP0; eauto. i. des.
+      eexists _, _, _, _. splits; [|eauto|eauto|].
+      * eapply rtc_internal_step_seq in STEPS.
+        eapply rtc_trans; [apply STEPS|eauto].
+      * apply rclo5_incl. auto.
+    + i. destruct th3_tgt, state.
+      exploit thread_step_deseq; eauto. i. des. simpl in *. subst.
+      exploit STEP; eauto. i. des.
+      destruct th2_src, state. destruct th3_src, state.
+      eexists _, _, _, _. splits; [| |eauto|].
+      * eapply rtc_internal_step_seq. eauto.
+      * eapply thread_step_seq. eauto.
+      * apply rclo5_step. eapply ctx_seq; eauto.
+        { apply rclo5_incl. eauto. }
+        { eapply _sim_stmts_mon; try apply rclo5_incl; eauto.
+          eapply _sim_stmts_mon; try apply LE; eauto.
+        }
+  - (* ite *)
+    ii. splits.
+    { i. inv TERMINAL_TGT. }
+    { i. simpl in *. subst. eexists _, _. splits; eauto. }
+    i. inv STEP_TGT; simpl in *.
+    + inv STEP; simpl in *; inv STATE.
+      eexists _, _, _, _. splits; eauto.
+      * econs 1. econs 5; eauto. econs.
+      * simpl. rewrite ? app_nil_r.
+        exploit COND; eauto. intro C. rewrite C.
+        destruct (RegFile.eval_expr rs_tgt cond_tgt).
+        { apply rclo5_incl. eauto. }
+        { apply rclo5_incl. eauto. }
+    + admit. (* declare *)
+    + inv STATE.
+  - (* dowhile *)
+    ii. splits.
+    { i. inv TERMINAL_TGT. }
+    { i. simpl in *. subst. eexists _, _. splits; eauto. }
+    i. inv STEP_TGT; simpl in *.
+    + inv STEP; simpl in *; inv STATE.
+      eexists _, _, _, _. splits; eauto.
+      * econs 1. econs 5; eauto. econs.
+      * apply rclo5_step. eapply ctx_seq.
+        { apply rclo5_incl. apply LE. eauto. }
+        ii. apply rclo5_step. eapply ctx_ite; eauto.
+        { ii. apply rclo5_step. eapply ctx_dowhile; eauto.
+          eapply _sim_stmts_mon; try apply rclo5_incl; eauto.
+          eapply _sim_stmts_mon; try apply LE; eauto.
+        }
+        { ii. apply rclo5_base; auto. }
+    + admit. (* declare *)
+    + inv STATE.
+Admitted.
+
+Definition sim_stmts := @_sim_stmts (paco5 (@_sim_thread lang <*> grespectful5 (@_sim_thread lang)) bot5).
+
+Lemma sim_stmts_nil sim_regs:
+  sim_stmts sim_regs [] [] sim_regs.
+Proof.
+  ii. pupto ctx_weak_respectful.
+Qed.
+
+Lemma sim_stmts_instr
+      (sim_regs:SIM_REGS) instr
+      (REGS: forall reg (REG: RegSet.mem reg (Instr.regs_of instr))
+               rs_src rs_tgt (RS: sim_regs rs_src rs_tgt),
+          rs_src reg = rs_tgt reg):
+  sim_stmts sim_regs [Stmt.instr instr] [Stmt.instr instr] sim_regs.
+Proof.
+  ii. pupto ctx_weak_respectful.
+Qed.
+
+Lemma sim_stmts_seq
+      sim_regs0 sim_regs1 sim_regs2
+      stmts1_src stmts2_src
+      stmts1_tgt stmts2_tgt
+      (SIM1: sim_stmts sim_regs0 stmts1_src stmts1_tgt sim_regs1)
+      (SIM2: sim_stmts sim_regs1 stmts2_src stmts2_tgt sim_regs2):
+  sim_stmts sim_regs0 (stmts1_src ++ stmts2_src) (stmts1_tgt ++ stmts2_tgt) sim_regs2.
+Proof.
+  ii. pupto ctx_weak_respectful.
+Qed.
+
+Lemma sim_stmts_ite
+      sim_regs0 sim_regs1
+      cond_src stmts1_src stmts2_src
+      cond_tgt stmts1_tgt stmts2_tgt
+      (COND: sim_expr sim_regs0 cond_src cond_tgt)
+      (SIM1: sim_stmts sim_regs0 stmts1_src stmts1_tgt sim_regs1)
+      (SIM2: sim_stmts sim_regs0 stmts2_src stmts2_tgt sim_regs1):
+  sim_stmts sim_regs0 [Stmt.ite cond_src stmts1_src stmts2_src] [Stmt.ite cond_tgt stmts1_tgt stmts2_tgt] sim_regs1.
+Proof.
+  ii. pupto ctx_weak_respectful.
+Qed.
+
+Lemma sim_stmts_dowhile
+      sim_regs
+      cond_src stmts_src
+      cond_tgt stmts_tgt
+      (COND: sim_expr sim_regs cond_src cond_tgt)
+      (SIM: sim_stmts sim_regs stmts_src stmts_tgt sim_regs):
+  sim_stmts sim_regs [Stmt.dowhile stmts_src cond_src] [Stmt.dowhile stmts_tgt cond_tgt] sim_regs.
+Proof.
+  ii. pupto ctx_weak_respectful.
+Qed.
